## ğŸ“ Summary

### The Complete Backpropagation Algorithm with Activations:

```
â”Œâ”€â”€â”€â”€â”€â”€â”€â”€â”€â”€â”€â”€â”€â”€â”€â”€â”€â”€â”€â”€â”€â”€â”€â”€â”€â”€â”€â”€â”€â”€â”€â”€â”€â”€â”€â”€â”€â”€â”€â”€â”€â”€â”€â”€â”€â”€â”€â”€â”€â”€â”€â”€â”€â”€â”€â”€â”€â”€â”€â”€â”€â”
â”‚                                                             â”‚
â”‚  1. FORWARD PASS:                                          â”‚
â”‚     â€¢ zâ‚ = Wâ‚Â·x + bâ‚                                      â”‚
â”‚     â€¢ hâ‚ = tanh(zâ‚)                                       â”‚
â”‚     â€¢ zâ‚‚ = Wâ‚‚Â·hâ‚ + bâ‚‚                                     â”‚
â”‚     â€¢ hâ‚‚ = tanh(zâ‚‚)                                       â”‚
â”‚     â€¢ zâ‚ƒ = Wâ‚ƒÂ·hâ‚‚ + bâ‚ƒ                                     â”‚
â”‚     â€¢ Å· = zâ‚ƒ                                              â”‚
â”‚                                                             â”‚
â”‚  2. COMPUTE LOSS:                                          â”‚
â”‚     â€¢ L = (Å· - y)Â²                                        â”‚
â”‚                                                             â”‚
â”‚  3. BACKWARD PASS (Compute Gradients):                    â”‚
â”‚     â€¢ âˆ‚L/âˆ‚Wâ‚ƒ = 2(Å· - y) Ã— hâ‚‚                             â”‚
â”‚     â€¢ âˆ‚L/âˆ‚bâ‚ƒ = 2(Å· - y)                                  â”‚
â”‚     â€¢ âˆ‚L/âˆ‚Wâ‚‚ = 2(Å· - y) Ã— Wâ‚ƒ Ã— (1-hâ‚‚Â²) Ã— hâ‚             â”‚
â”‚     â€¢ âˆ‚L/âˆ‚bâ‚‚ = 2(Å· - y) Ã— Wâ‚ƒ Ã— (1-hâ‚‚Â²)                  â”‚
â”‚     â€¢ âˆ‚L/âˆ‚Wâ‚ = 2(Å·-y) Ã— Wâ‚ƒ Ã— (1-hâ‚‚Â²) Ã— Wâ‚‚ Ã— (1-hâ‚Â²) Ã— x â”‚
â”‚     â€¢ âˆ‚L/âˆ‚bâ‚ = 2(Å·-y) Ã— Wâ‚ƒ Ã— (1-hâ‚‚Â²) Ã— Wâ‚‚ Ã— (1-hâ‚Â²)    â”‚
â”‚                                                             â”‚
â”‚  4. UPDATE PARAMETERS:                                     â”‚
â”‚     â€¢ Wâ‚ƒ â† Wâ‚ƒ - Î± Ã— (âˆ‚L/âˆ‚Wâ‚ƒ)                             â”‚
â”‚     â€¢ bâ‚ƒ â† bâ‚ƒ - Î± Ã— (âˆ‚L/âˆ‚bâ‚ƒ)                             â”‚
â”‚     â€¢ Wâ‚‚ â† Wâ‚‚ - Î± Ã— (âˆ‚L/âˆ‚Wâ‚‚)                             â”‚
â”‚     â€¢ bâ‚‚ â† bâ‚‚ - Î± Ã— (âˆ‚L/âˆ‚bâ‚‚)                             â”‚
â”‚     â€¢ Wâ‚ â† Wâ‚ - Î± Ã— (âˆ‚L/âˆ‚Wâ‚)                             â”‚
â”‚     â€¢ bâ‚ â† bâ‚ - Î± Ã— (âˆ‚L/âˆ‚bâ‚)                             â”‚
â”‚                                                             â”‚
â”‚  5. REPEAT until convergence                               â”‚
â”‚                                                             â”‚
â””â”€â”€â”€â”€â”€â”€â”€â”€â”€â”€â”€â”€â”€â”€â”€â”€â”€â”€â”€â”€â”€â”€â”€â”€â”€â”€â”€â”€â”€â”€â”€â”€â”€â”€â”€â”€â”€â”€â”€â”€â”€â”€â”€â”€â”€â”€â”€â”€â”€â”€â”€â”€â”€â”€â”€â”€â”€â”€â”€â”€â”€â”˜
```

---

## ğŸ”— Connection to Code

In Python/NumPy, the backward pass would look like:

```python
def backward_with_tanh(x, y, y_pred, h1, h2, z1, z2, W3, W2, learning_rate=0.01):
    """
    Compute gradients and update parameters for 3-layer network with tanh.
    """
    n = len(x)  # batch size
    
    # Error signal
    error = y_pred - y
    
    # Activation derivatives
    tanh_deriv_2 = 1 - h2**2  # (1 - tanhÂ²(zâ‚‚))
    tanh_deriv_1 = 1 - h1**2  # (1 - tanhÂ²(zâ‚))
    
    # Layer 3 gradients (no activation)
    dW3 = (2.0 / n) * np.sum(error * h2)
    db3 = (2.0 / n) * np.sum(error)
    
    # Layer 2 gradients (with tanh)
    dz2 = error * W3 * tanh_deriv_2
    dW2 = (2.0 / n) * np.sum(dz2 * h1)
    db2 = (2.0 / n) * np.sum(dz2)
    
    # Layer 1 gradients (with tanh)
    dz1 = dz2 * W2 * tanh_deriv_1
    dW1 = (2.0 / n) * np.sum(dz1 * x)
    db1 = (2.0 / n) * np.sum(dz1)
    
    # Update parameters
    W3 -= learning_rate * dW3
    b3 -= learning_rate * db3
    W2 -= learning_rate * dW2
    b2 -= learning_rate * db2
    W1 -= learning_rate * dW1
    b1 -= learning_rate * db1
    
    return W3, b3, W2, b2, W1, b1
```

---
